\subsection{Subject Reduction}
\label{subsec:subject-reduction}
\emph{Subject reduction}, also sometimes referred to as ``type preservation'', ensures that if a program has a specific type, then the program will have the same type after a reduction step.
Before we present the subject reduction proof, we first introduce a number of useful lemmas.

\input{Chapters/MetaTheory//lemmas.tex}

In many reduction cases, there are values on the stack that get consumed by reducing an instruction.
This creates a bit of a problem because those values represent intermediate state, and as such will introduce new index variables to the index type context in their postcondition.
After reduction, the intermediate state is no longer present, so we lose those index variables from the postconditions.

For example, $(t.\<const> c)\; \<drop>$ could be typed as $\epsilon;l;\phi \rightarrow \epsilon;l;\phi,\ti{t}{a},(= a\; \ti{t}{c})$ where $a$ represent the value on the stack $t.\<const> c$.
This would reduce to $\epsilon$, and then we lose the information about $a$ in the postcondition index type system.
However, this can be solved using implication, as we know $a$ is fresh from the const rule, and therefore we allow saying $\phi \implies \phi,\ti{t}{a},(= a\; \ti{t}{c})$ after reduction.
This pattern will appear in any case of the proof that consumes values.

\begin{theorem}{Subject Reduction}
  If $\vdash_i s;v^{*};e^{*} : ti^{*};l;\phi$ and $s;v^{*};e^{*} \hookrightarrow_i s';v'^{*};e'^{*}$ then $\vdash_i s';v'^{*};e'^{*} : ti^{*};l;\phi$.
\end{theorem}
\begin{proof}
By case analysis on the reduction rules.

\begin{itemize}
    %% Binop -> const
    \item $C\vdash (t.\<const> c_1)\; (t.\<const> c_2)\; t.binop : ti_1^{*};l_1;\phi_1 \rightarrow ti_2^{*};l_2;\phi_2$
    \\ $\land$ $(t.\<const> c_1)\; (t.\<const> c_2)\; t.binop \hookrightarrow t.\<const> c$ where $c=binop(c_1,c_2)$

        By $inversion$ on $const$ and $binop$, we know that $ti_2^{*} = ti_1^{*} \ti{t}{a_3}$, $l_2=l_1$, and that
        \begin{align*}
            \phi_1&,
            \begin{stackTL}
                \ti{t}{a_1}, (= a_1\; \ti{t}{c_1}), \\
                \ti{t}{a_2}, (= a_2\; \ti{t}{c_2}), \\
                \ti{t}{a_3}, (= a_3\; (binop\; a_1\; a_2))
            \end{stackTL} \\
            &\implies \phi_2
        \end{align*}

        By $const$, $C \vdash t.\<const> c :
            \begin{stackTL}
                \epsilon;l_1;\phi_1 \\
                \rightarrow \ti{t}{a_3};l_1;g_1;\phi_1,\ti{t}{a_3},(\<eq> a_3\;\ti{t}{c})
            \end{stackTL}$.

        Because $c=binop_t(c_1,c_2)$, then by $\implies$,
        \begin{align*}
            \phi_1,\ti{t}{a},(= a\; \ti{t}{c}) &\implies \phi_1,
            \begin{stackTL}
                \ti{t}{a_1}, (= a_1\; \ti{t}{c_1}), \\
                \ti{t}{a_2}, (= a_2\; \ti{t}{c_2}), \\
                \ti{t}{a_3}, (= a_3\; (binop\; a_1 a_2))
            \end{stackTL}
        \end{align*}

        Therefore, $C \vdash (t.\<const> c) : ti_1^{*};l_1;\phi_1 \rightarrow ti_1^{*}\; \ti{t}{a_3};l_1;\phi_2$, by $stack-poly$ and $sub-typing$

    %% Binop -> trap
    \item  $C\vdash (t.\<const> c_1)\; (t.\<const> c_2)\; t.binop : ti_1^{*};l_1;\phi_1 \rightarrow ti_2^{*};l_2;\phi_2$
    \\ $\land$ $(t.\<const> c_1)\; (t.\<const> c_2)\; t.binop \hookrightarrow \<trap>$

        Trivially, $C\vdash \<trap> : ti_1^{*};l_1;\phi_1 \rightarrow ti_2^{*};l_2;\phi_2$ by $trap$.

    %% Relop
    \item $C\vdash (t.\<const> c_1)\; (t.\<const> c_2)\; t.relop : ti_1^{*};l_1;\phi_1 \rightarrow ti_2^{*};l_2;\phi_2$
    \\ $\land$ $(t.\<const> c_1)\; (t.\<const> c_2)\; t.relop \hookrightarrow t.\<const> c$ where $c=relop(c_1,c_2)$

        Similar to $binop$.

    %% Testop
    \item $C\vdash (t.\<const> c)\; t.testop : ti_1^{*};l_1;\phi_1 \rightarrow ti_2^{*};l_2;\phi_2$
    \\ $\land$ $(t.\<const> c)\; t.testop \hookrightarrow \<ithreetwo>.\<const> c_2$ where $c_2=testop(c)$

        \todo{This is wonky}

        By $inversion$ on $const$ and $testop$, we know that $ti_2^{*}=ti_1^{*}\; \ti{t}{a_2}$, $l_2=l_1$, and that
        \begin{align*}
            \phi_1&,
            \begin{stackTL}
                \ti{t}{a_1}, (= a_1\;\ti{t}{c}), \\
                \ti{\<ithreetwo>}{a_2}, (= a_2\;(testop\;a_1))
            \end{stackTL} \\
            &\implies \phi_2
        \end{align*}

        By $const$, $C \vdash t.\<const> c :
            \begin{stackTL}
                \epsilon;l_1;g_1;\phi_1 \\
                \rightarrow \ti{\<ithreetwo>}{a_2};l_1;\phi_1,\ti{\<ithreetwo>}{a_2},(= a_2\;\ti{t}{c_2})
            \end{stackTL}$.

        Because $c_2=testop_t(c)$, then by $\implies$,
        \begin{align*}
            \phi_1,\ti{t}{a},(= a\;\ti{t}{c_2}) &\implies \phi_1,
            \begin{stackTL}
                \ti{t}{a_1}, (= a_1\;\ti{t}{c}), \\
                \ti{\<ithreetwo>}{a_2}, (= a_2\;(testop\;a_1))
            \end{stackTL}
        \end{align*}

    %% Unreachable
    \item $C\vdash \<unreachable> : ti_1^{*};l_1;\phi_1 \rightarrow ti_2^{*};l_2;\phi_2$
    \\ $\land$ $\<unreachable> \hookrightarrow \<trap>$

        Trivially, $C\vdash \<trap> : ti_1^{*};l_1;\phi_1 \rightarrow ti_2^{*};l_2;\phi_2$ by $trap$.

    %% Nop
    \item $C\vdash \<nop> : ti_1^{*};l_1;\phi_1 \rightarrow ti_2^{*};l_2;\phi_2$
    \\ $\land$ $\<nop> \hookrightarrow \epsilon$

        By $inversion$ on $nop$, we know that $ti_2^{*} = ti_1^{*}$, $l_2 = l_1$, and $\phi_1 \implies \phi_0$ and $\phi_0 \implies \phi_2$ for some $\phi_0$.

        $C\vdash \epsilon : \epsilon;l;g;\phi_0 \rightarrow \epsilon;l;g;\phi_0$ by $empty$.

        Then, $C \vdash \epsilon ti_1^{*};l;g;\phi_1 \rightarrow ti_1^{*};l;g;\phi_2$ by $stack-poly$ and $sub-typing$.

    %% Drop
    \item $C\vdash (t.\<const> c)\; \<drop> : ti_1^{*};l_1;\phi_1 \rightarrow ti_2^{*};l_2;\phi_2$
    \\ $\land$ $(t.\<const> c)\; \<drop> \hookrightarrow \epsilon$

        By $inversion$ on $compostion$, $const$, and $drop$, we know that $ti_2^{*} = ti_1^{*}$, $l_2 = l_1$, and $\phi_1 \implies \phi_0$ and $\phi_0 \implies \phi_2$ for some $\phi_0$.

        By $empty$, $C\vdash \epsilon : \epsilon;l_1;\phi_0 \rightarrow \epsilon;l_1;\phi_0$.

        Then, $C\vdash \epsilon : ti_1^{*};l_1;\phi_1 \rightarrow ti_1^{*};l_1;\phi_2$ by $stack-poly$ and $sub-typing$.

    %% Select
    \item Case: $C\; {\begin{stackTL}
        \vdash (t.\<const> c_1)\;(t.\<const> c_2)\;(\<ithreetwo>.\<const> 0)\;\<select>
        \\ : ti_1^{*};l_1;\phi_1 \rightarrow ti_2^{*};l_2;\phi_2
    \end{stackTL}}$
    \\ $\land$ $(t.\<const> c_1)\;(t.\<const> c_2)\;(\<ithreetwo>.\<const> 0)\;\<select> \hookrightarrow (t.\<const> c_2)$

        By $const$ and $select$, we know that $ti_2^{*} = ti_1^{*}\;\ti{a_3}$, $l_2 = l_1$, and
        $
        {\begin{stackTL}
            \phi_1, {\begin{stackTL}
                \ti{t}{a_1}, (= a_1\;\ti{t}{c_1}), \\
                \ti{t}{a_2}, (= a_2\;\ti{t}{c_2}), \\
                \ti{\<ithreetwo>}{a}, (= a\;\ti{\<ithreetwo>}{0}), \\
                \ti{t}{a_3},(if\; (= a\; \ti{\<ithreetwo>}{0})\; (= a_3\; a_2)\; (= a_3\; a_1))
            \end{stackTL}} \\
            \implies \phi_2
        \end{stackTL}}
        $

        By $const$, \\
        $ C \vdash (t.\<const> c_2) :
            {\begin{stackTL}
                \epsilon;l_1;\phi_1 \\
                \rightarrow \ti{t}{a_3};l_1;\phi_1,\ti{t}{a_3},(= a_3\; \ti{t}{c_2}) \\
            \end{stackTL}} $

        $C \vdash (t.\<const> c_2) : ti_1^{*};l_1;\phi_1 \rightarrow ti_1^{*}\;\ti{t}{a_3};l_1;\phi_1,\ti{t}{a_3},(= a_3 \; \ti{t}{c_2})$ by $stack-poly$.

        By $\implies$, we have \\
        $\phi_1,\ti{t}{a_3},(\<eq> a_3\; \ti{t}{c_2}) \implies \phi_1, {\begin{stackTL}
            \ti{t}{a_1}, (\<eq> a_1\; \ti{t}{c_1}), \\
            \ti{t}{a_2}, (\<eq> a_2\; \ti{t}{c_2}), \\
            \ti{\<ithreetwo>}{a}, (= a\;\ti{\<ithreetwo>}{0}), \\
            \ti{t}{a_3},(if\; (= a\; \ti{\<ithreetwo>}{0})\; (= a_3\; a_2)\; (= a_3\; a_1))
        \end{stackTL}} \\ $

        Therefore,
        $ C \vdash (t.\<const> c_2) :
        ti_1^{*};l_1;\phi_1
            \rightarrow ti_2^{*}\;\ti{t}{a_3};l_1;\phi_2$ by $sub-typing$

    %% Block
    \item Case: $C \vdash v^n \; \<block> tfi \; e^{*} \<end> : ti_1^{*};l_1;\phi_1 \rightarrow ti_2^{*};l_2;\phi_2$
    \\ $\land$ $v^n \; \<block> tfi \; e^{*} \<end> \hookrightarrow \<label>_m \{ \epsilon \} \; v^n \; e^{*} \<end>$

        Let $ti_3^n;l_3;\phi_3 \rightarrow ti_4^m;l_4;\phi_4=tfi$, $(t.\<const> c)^n=v^n$.

        $C \vdash \<block> tfi \; e^{*} \<end> : ti_1^{*}\; \ti{t}{a}^n;l_1;\phi_1,\ti{t}{a}^n,(\<eq> a \; \ti{t}{c})^n \rightarrow ti_2^{*};l_2;\phi_2$ by $inversion$ on $composition$ and $const$.

        Therefore, by $inversion$ on $block$, $l_1=l_3$ and $l_2=l_4$. We will use $l_1,l_2$ in place of $l_3,l_4$, respectively, for the remainder of the proof case.

        Further, $\ti{t}{a}^n=ti_3^n$, $ti_2^{*}=ti_1^{*}\; ti_4^m$, $\phi_1,\ti{t}{a}^n,(\<eq> a \; \ti{t}{c})^n \implies \phi_3$, and $\phi_4 \implies \phi_2$ by $inversion$ on $block$.

        $C,\text{label}(t_4^{m};l_2;\phi_4) \vdash (t.\<const> c)^n : \epsilon;l_1;\phi_1 \rightarrow \\ \ti{t}{a}^n;l_1;\phi_1,\ti{t}{a}^n,(\<eq> a \; \ti{t}{c})^n$ by $const$.

        $C,\text{label}(t_4^{m};l_2;g_2;\phi_4) \vdash (t.\<const> c)^n : \epsilon;l_1;\phi_1 \rightarrow \\ \ti{t}{a}^n;l_1;\phi_3$ by $sub-typing$.

        $C,\text{label}(t_4^{m};l_2;\phi_4) \vdash e^{*} : \ti{t}{a}^n;l_1;\phi_3 \rightarrow ti_4^m;l_2;\phi_4$ because it is a sub-derivation of $block$ which we have already assumed to hold.

        Then $C,\text{label}(t_4^{m};l_2;\phi_4) \vdash (t.\<const> c)^n\; e^{*} : \epsilon;l_1;\phi_1 \rightarrow \\ ti_4^m;l_2;\phi_4$ by $composition$.

        By $empty$ and $stack-poly$, $C \vdash \epsilon : ti_2^m;l_2;\phi_4 \rightarrow ti_2^m;l_2;\phi_4$.

        Therefore, $C \vdash \<label>_m \{ \epsilon \} \; v^n \; e^{*} \<end> : \epsilon;l_1;\phi_1 \rightarrow ti_2^m;l_2;\phi_4$ by $label$.

        $C \vdash \<label>_m \{ \epsilon \} \; v^n \; e^{*} \<end> : ti_1^{*};l_1;\phi_1 \rightarrow ti_1^{*}\; ti_4^m;l_2;\phi_2$ by $stack-poly$ and $sub-typing$.

    \item Case: $C \vdash v^n \; \<loop> tfi \; e^{*} \<end> : ti_1^{*};l_1;\phi_1 \rightarrow ti_2^{*};l_2;\phi_2$
    \\ $\land$ $v^n \; \<loop> tfi \; e^{*} \<end> \hookrightarrow \<label>_n \{ \<loop> tfi \; e^{*} \<end> \} \; v^n \; e^{*} \<end>$

        Let $ti_3^n;l_3;\phi_3 \rightarrow ti_4^m;l_4;\phi_4=tfi$, $(t.\<const> c)^n=v^n$.

        $C \vdash \<loop> tfi \; e^{*} \<end> : ti_1^{*}\; \ti{t}{a}^n;l_1;\phi_1,\ti{t}{a}^n,(\<eq> a \; \ti{t}{c})^n \rightarrow ti_2^{*};l_2;g_2;\phi_2$ by $inversion$ on $composition$ and $const$.

        Therefore, by $inversion$ on $loop$, $l_1=l_3$ and $l_2=l_4$. We will use $l_1,l_2$ in place of $l_3,l_4$, respectively, for the remainder of the proof case.

        Further, $\ti{t}{a}^n=ti_3^n$, $ti_2^{*}=ti_1^{*}\; ti_4^m$, $\phi_1,\ti{t}{a}^n,(\<eq> a \; \ti{t}{c})^n \implies \phi_3$, and $\phi_4 \implies \phi_2$ by $inversion$ on $loop$.

        $C,\text{label}(t_3^{n};l_1;\phi_3) \vdash (t.\<const> c)^n : \epsilon;l_1;\phi_1 \rightarrow \\ \ti{t}{a}^n;l_1;\phi_1,\ti{t}{a}^n,(\<eq> a \; \ti{t}{c})^n$ by $const$.

        $C,\text{label}(t_3^{n};l_1;\phi_3) \vdash (t.\<const> c)^n : \epsilon;l_1;\phi_1 \rightarrow \\ \ti{t}{a}^n;l_1;\phi_3$ by $sub-typing$.

        $C,\text{label}(t_3^{n};l_1;\phi_3) \vdash e^{*} : ti_1^n;l_1;\phi_3 \rightarrow ti_2^m;l_1;\phi_4$ because it is a sub-derivation of $loop$ which we have already assumed to hold.

        Then $C,\text{label}(t_3^{n};l_1;\phi_3) \vdash (t.\<const> c)^n\; e^{*} : \epsilon;l_1;\phi_1 \rightarrow \\ ti_4^m;l_2;\phi_4$ by $composition$.

        $C \vdash \<loop> tfi \; e^{*} \<end> : \ti{t}{a}^n;l_1;\phi_1,\ti{t}{a}^n,(\<eq> a \; \ti{t}{c})^n \rightarrow ti_4^{m};l_2;g_2;\phi_4$ by $loop$.

        Therefore, $C \vdash \<label>_m \{ \<loop> tfi \; e^{*} \<end> \} \; v^n \; e^{*} \<end> : \epsilon;l_1;\phi_1 \rightarrow ti_4^m;l_2;\phi_4$ by $label$.

        $C \vdash \<label>_m \{ \epsilon \} \; v^n \; e^{*} \<end> : ti_1^{*};l_1;\phi_1 \rightarrow ti_2^{*};l_2;\phi_2$ by $stack-poly$ and $sub-typing$.

    \item Case: $C \vdash (\<ithreetwo>.\<const> 0) \; \<if> tfi \; e_1^{*} \<else> e_2^{*} \<end> : ti_1^{*};l_1;\phi_1 \rightarrow ti_2^{*};l_2;\phi_2$
    \\ $\land$ $(\<ithreetwo>.\<const> 0) \; \<if> tfi \; e_1^{*} \<else> e_2^{*} \<end> \hookrightarrow \<block> tfi \; e_2^{*} \<end>$

        Let $tfi = ti_3^n \; \ti{<ithreetwo>}{a};l_3;\phi_3 \rightarrow ti_4^m;l_4;\phi_4$, \\ $tfi_1 = ti_3^n;l_3;\phi_3,\neg(= a\; \ti{\<ithreetwo>}{0}) \rightarrow ti_4^m;l_4;\phi_4$, \\
        and $tfi_2 = ti_3^n;l_3;\phi_3,(= a\; \ti{\<ithreetwo>}{0}) \rightarrow ti_4^m;l_4;\phi_4$.

        By $inversion$ on $composition$, $const$, and $if$, $ti_1^{*}=ti_0^{*}\; ti_3^{n}$ and $ti_2^{*}=ti_0^{*} \; ti_4^{m}$ for some $ti_0^{*}$, $l_1=l_3$, $l_2=l_4$, $\phi_1,\ti{\<ithreetwo>}{a},(\<eq> a\; 0) \implies \phi_3$, and $\phi_4 \implies \phi_2$.

        $C,\text{label}(ti_4^m;l_4;\phi_4) \vdash e_2^{*} : tfi_2$ because it is a sub-derivation of $if$ which we have assumed to hold.

        Then, $C \vdash \<block> tfi_2 \; e_2^{*} \<end>$ by $block$.

        Since $a$ is fresh after reduction, $\phi_1 \implies \phi_1,\ti{t}{a},(\<eqz> a)$ by $\implies$.

        Therefore, $C \vdash \<block> tfi_2\; e_2^{*} \<end> : \\ ti_0^{*}\; ti_3^n;l_1;\phi_1,\ti{t}{a},(\<eqz> a) \rightarrow s\; ti_0^{*}\;ti_4^m;l_2;\phi_2$ by $extension$ and $sub-typing$.

    \item Case: $C \vdash (\<ithreetwo>.\<const> k+1) \; \<if> tfi \; e_1^{*} \<else> e_2^{*} \<end> : ti_1^{*};l_1;\phi_1 \rightarrow ti_2^{*};l_2;\phi_2$
    \\ $\land$ $(\<ithreetwo>.\<const> k+1) \; \<if> tfi \; e_1^{*} \<else> e_2^{*} \<end> \hookrightarrow \<block> tfi \; e_1^{*} \<end>$

        Similar to above.

    \item Case: $C \vdash \<label>_n \{ e^{*} \} \; v^n \<end> : ti_1^{*};l_1;\phi_1 \rightarrow ti_2^{*};l_2;\phi_2$
    \\ $\land$ $\<label>_n \{ e^{*} \} \; v^n \<end> \hookrightarrow v^n$

        $C \vdash \<label>_n \{ e^{*} \} \; v^n \<end> : \epsilon;l_1;\phi_1 \rightarrow ti_4^{n};l_2;\phi_2$ by $inversion$ on $label$.

        By $inversion$, we know $ti_2^{*}=ti_1^{*}\;ti_4^{n}$.

        $C \vdash v^n : \epsilon;l_1;\phi_1 \rightarrow ti_4^{n};l_2;\phi_2$ because it is a premise of $label$ which we have assumed to hold.

        Therefore, $C \vdash v^n : ti_1^{*};l_1;\phi_1 \rightarrow ti_1^{*}\;ti_4^{n};l_1;\phi_2$ by $stack-poly$.

    \item Case: $C \vdash \<label>_n \{ e^{*} \} \; \<trap> \<end> : ti_1^{*};l_1;\phi_1 \rightarrow ti_2^{*};l_2;\phi_2$
    \\ $\land$ $\<label>_n \{ e^{*} \} \; \<trap> \<end> \hookrightarrow \<trap>$

        Trivially, $C\vdash \<trap> : ti_1^{*};l_1;\phi_1 \rightarrow ti_2^{*};l_2;\phi_2$ by $trap$.

    \item Case: $C \vdash \<label>_n \{ e^{*} \} \; L^j [v^n \; (\<br> j)] \<end> : ti_1^{*};l_1;\phi_1 \rightarrow ti_2^{*};l_2;\phi_2$
    \\ $\land$ $\<label>_n \{ e^{*} \} \; L^j [v^n \; (\<br> j)] \hookrightarrow v^n \; e^{*}$

        By $inversion$, $ti_2^{*}=ti_1^{*}\;ti_4^{*}$.

        Let $(t.\<const> c)^n = v^n$.

        $C,\text{label}(ti_1^n;l_3;\phi_5)^j \vdash v^n\; (\<br> j) : \epsilon;l_3;\phi_3 \rightarrow ti_\emptyset^{*};l_\emptyset;\phi_\emptyset$ for some $l_3$ and $\phi_3$, where $\phi_5=\phi_3,\ti{t}{a}^n,(= a\; \ti{t}{c})^n$, by $inversion$ on $label$ and $br$.

        $C,\text{label}(ti_1^n;l_3;\phi_5)^j \vdash (\<br> j) : ti_1^n;l_3;\phi_5 \rightarrow ti_\emptyset^{*};l_\emptyset;\phi_\emptyset$, by $inversion$ on $composition$ and $const$.

        Then, $C,\text{label}(ti_1^n;l_3;\phi_5)^j \vdash v^n : \epsilon;l_3;\phi_3 \rightarrow ti_1^n;l_3;\phi_5$ since it is a premise of $composition$ which we have assumed to hold.

        $C \vdash e^{*} : ti_1^n;l_3;\phi_5 \rightarrow ti_2^{*};l_2;\phi_4$ since it is a premise of $label$ which we have assumed to hold, and $\phi_4 \implies \phi_2$ by $inversion$ on $label$.

        Then, $C \vdash v^n \; e^{*} : \epsilon;l_1;\phi_1 \rightarrow ti_2^{*};l_2;\phi_4$ by $nested-type-preserved$ and $composition$.

        Finally, $C \vdash v^n \; e^{*} : ti_1^{*};l_1;\phi_1 \rightarrow ti_1^{*}\;ti_4^{*};l_2;\phi_2$ by $stack-poly$ and $sub-typing$.

    \item Case: $C \vdash (\<ithreetwo>.\<const> 0)\;(\<brif> j) : ti_1^{*};l_1;\phi_1 \rightarrow ti_2^{*};l_2;\phi_2$
    \\ $\land$ $(\<ithreetwo>.\<const> 0)\;(\<brif> j) \hookrightarrow \epsilon$

        $ti_1^{*}=ti_2^{*}$, $l_1=l_2$, and $\phi_1,\ti{\<ithreetwo>}{a},(\<eq> a\; \ti{\<ithreetwo>}{0}),(\<eqz> a) \implies \phi_2$ by $inversion$ on $composition$, $const$, and $br \_ if$.

        $C \vdash \epsilon : \epsilon;l_1;\phi_1 \rightarrow \epsilon;l_1;\phi_1$ by $empty$.

        $C \vdash \epsilon : ti_1^{*};l_1;\phi_1 \rightarrow ti_1^{*};l_1;\phi_1$ by $stack-poly$.

        $\phi_1 \implies \phi_1,\ti{\<ithreetwo>}{a},(\<eq> a\; \ti{\<ithreetwo>}{0}),(\<eqz> a)$ because $a$ is fresh after reduction, and therefore $\phi_1 \implies \phi_2$.

        Then, $C \vdash \epsilon : ti_1^{*};l_1;\phi_1 \rightarrow ti_1^{*};l_1;\phi_2$ by $sub-typing$.

    \item Case: $C \vdash (\<ithreetwo>.\<const> k+1)\;(\<brif> j) : ti_1^{*};l_1;\phi_1 \rightarrow ti_2^{*};l_2;\phi_2$
    \\ $\land$ $(\<ithreetwo>.\<const> k+1)\;(\<brif> j) \hookrightarrow \<br> j$

        $C_label(j)=ti_1^{*};l_1;\phi_1,\ti{t}{a},\neg(\<eqz> a)$ because it is a side condition of $br\_if$ which we have assumed to hold.

        $C \vdash \<br> j : ti_1^{*};l_1;\phi_1,\ti{t}{a},\neg(\<eqz> a) \rightarrow ti_2^{*};l_2;\phi_2$ by $br$.

        Because $a$ is fresh after reduction, $\phi_1 \implies \phi_1,\ti{\<ithreetwo>}{a},\neg(\<eqz> a)$.

        Therefore, $C \vdash \<br> j : ti_1^{*};l_1;\phi_1 \rightarrow ti_2^{*};l_2;\phi_2$ by $sub-typing$.

    \item Case: $C \vdash (\<ithreetwo>.\<const> k)\;(\<brtable> j_1^k\; j\; j_2^{*}) : ti_1^{*};l_1;\phi_1 \rightarrow ti_2^{*};l_2;\phi_2$
    \\ $\land$ $(\<ithreetwo>.\<const> k)\;(\<brtable> j_1^k\; j\; j_2^{*}) \hookrightarrow \<br> j$

        By $inversion$, we know that $C_\text{label}(j) = ti^{*};l_1;\phi_3$, $ti_1^{*} = ti_0^{*} \; ti^{*}$ for some $ti_0^{*}$, and $phi_1 \implies \phi_3$.

        $C \vdash \<br> j : ti_1^{*};l_1;\phi_3 \rightarrow ti_2^{*};l_2;\phi_2$ by $br$.

        $C \vdash \<br> j : ti_1^{*};l_1;\phi_1 \rightarrow ti_2^{*};l_2;\phi_2$ by $sub-typing$.

    \item Case: $C \vdash (\<ithreetwo>.\<const> k+n)\;(\<brtable> j_1^k\; j) : ti_1^{*};l_1;\phi_1 \rightarrow ti_2^{*};l_2;\phi_2$
    \\ $\land$ $(\<ithreetwo>.\<const> k+n)\;(\<brtable> j_1^k\; j) \hookrightarrow \<br> j$

        By $inversion$, we know that $C_\text{label}(j) = ti^{*};l_1;\phi_3$, $ti_1^{*} = ti_0^{*} \; ti^{*}$ for some $ti_0^{*}$, and $phi_1 \implies \phi_3$.

        $C \vdash \<br> j : ti_1^{*};l_1;\phi_3 \rightarrow ti_2^{*};l_2;\phi_2$ by $br$.

        $C \vdash \<br> j : ti_1^{*};l_1;\phi_1 \rightarrow ti_2^{*};l_2;\phi_2$ by $sub-typing$.

    \item Case: $S;C \vdash \<call> j : ti_1^{*};l_1;\phi_1 \rightarrow ti_2^{*};l_2;\phi_2$
    \\ $\land$ $s;\<call> j \hookrightarrow_i \<call> s_\text{func}(i,j)$

        By $inversion$, we know that $l_2 = l_1$, $ti_1^{*} = ti^{*} \; ti_3^{*}$, $ti_1^{*} = ti^{*} \; ti_4^{*}$, $\phi_1 \implies \phi_3$, and $\phi_3,\phi_4 \implies \phi_2$, where $ti_3^{*};l_3;\phi_3 \rightarrow ti_4^{*};l_4;\phi_4 = C_\text{func}(j)$.

        We know $S \vdash s_\text{inst}(i) : C$ since it is a premise of $\vdash s : S$ which we have assumed to hold.

        Then we know $S \vdash s_\text{func}(i,j) : ti_3^{*};l_3;\phi_3 \rightarrow ti_4^{*};l_4;\phi_4$ because it is a premise of $S \vdash s_\text{inst}(i) : C$.

        Therefore, $S;C\vdash \<call> s_\text{func}(i,j) : ti_3^{*};l_3;\phi_3 \rightarrow ti_4^{*};l_4;\phi_4$ by $call-cl$.

        $S;C\vdash \<call> s_\text{func}(i,j) : ti_1^{*};l_1;\phi_1 \rightarrow ti_2^{*};l_2;\phi_2$ by $stack-poly$ and $sub-typing$.

    \item Case: $S;C \vdash_i (\<ithreetwo>.\<const> j)\; \<callindirect> tfi : ti_1^{*};l_1;\phi_1 \rightarrow ti_2^{*};l_2;\phi_2$
    \\ $\land$ $s;(\<ithreetwo>.\<const> j)\; \<callindirect> tfi \hookrightarrow_i \<call> s_\text{tab}(i,j)$ where $s_\text{tab}(i,j)_\text{code}=(\<func> tfi_0\; \<local>\; t^{*}\; e^{*})$ and $tfi_0 <: tfi$

        Let $ti_3^{*};l_3;\phi_3 \rightarrow ti_4^{*};l_4;\phi_4 = tfi$

        By $inversion$ on $composition$, $const$, and $call-indirect$, we know that $ti_1^{*}=ti_0^{*}\; ti_3^{*}$ and $ti_2^{*}=ti_0^{*}\; ti_4^{*}$ for some $ti_0^{*}$, $l_1=l_3$, $l_2=l_4$, $\phi_1 \implies \phi_3$, and $\phi_4 \implies \phi_2$.

        $S \vdash s_\text{tab}(i,j) : tfi_0$ since it is a premise of $\vdash s : S$ which we have assumed to hold.

        Then, $S;C \vdash_i \<call> s_\text{tab}(i,j) : tfi_0$ by $call-cl$.

        $S;C \vdash_i \<call> s_\text{tab}(i,j) : tfi$ by $sub-typing$.

        Therefore, $S;C \vdash_i \<call> s_\text{tab}(i,j) : ti_0^{*}\;ti_1^{*};l_1;\phi_1 \rightarrow ti_0^{*}\;ti_1^{*};l_2;\phi_2$ by $stack-poly$.

    \item Case: $S;C \vdash_i (\<ithreetwo>.\<const> j)\; \<callindirect> tfi : ti_1^{*};l_1;\phi_1 \rightarrow ti_2^{*};l_2;\phi_2$
    \\ $\land$ $s;(\<ithreetwo>.\<const> j)\; \<callindirect> tfi \hookrightarrow_i \<trap>$.

        Trivially, $S;C \vdash_i \<trap> : ti_1^{*};l_1;\phi_1 \rightarrow ti_2^{*};l_2;\phi_2$ by $trap$.

    \item Case: $S;C \vdash_i v^n\; \<call> cl : ti_1^{*};l_1;\phi_1 \rightarrow ti_2^{*};l_2;\phi_2$
    \\ $\land$ $s;v^n\; \<call> cl \hookrightarrow_i \<local>_m\{j;v^n \; (t.\<const> 0)^k\} \; \<block> tfi_1\; e^{*} \<end> \<end>$
    \\ where $cl_\text{code} = \<func> tfi_2\; \<local>\; t^k \; e^{*}$ and $cl_\text{inst} = j$

        \todo{This needs an overhaul}

        Let $tfi_0 = ti_1^{*};l_1;\phi_1 \rightarrow ti_2^{*};l_2;\phi_2$, $tfi_1 = \epsilon;l_3;\phi_3 \rightarrow ti_4^{m};l_4;\phi_4$, and $tfi_2 = ti_3^{n};\ti{t_2}{a_2}^{n}\; \ti{t}{a}^k;\phi_3,\ti{t}{a}^k,(= a \;\ti{t}{0})^k \rightarrow ti_4^{m};l_4;\phi_4$ by $inversion$.

        $S;C \vdash (t_2 \<const> c)^n : ti_1^{*};l_1;\phi_1 \rightarrow ti_1^{*}\;ti_5^n;l_1;\phi_1,\ti{t_2}{a_2},(= a_2 \; \ti{t_2}{c})$, where $v^n=(t_2 \<const> c)^n$,
        and $S;C\vdash \<call> cl : ti_1^{*}\;ti_5^n;l_1;\phi_1,\ti{t_2}{a_2}^{n},(= a_2 \; \ti{t_2}{c})^{n} \rightarrow ti^{*}\;ti_2^m;l_2;\phi_2$ because they are premises of $composition$ which we have assumed to hold.

        By inversion, $l_2=l_1$, $ti_2^{*}=ti_1^{*}\;ti_4^m$, $\phi_1,\ti{t_2}{a_2},(\<eq> a_2 \; \ti{t_2}{c}) \implies \phi_3$, $\phi_4 \implies \phi_2$, and $S\vdash cl : tfi_1$.

        Therefore, $C \vdash \<func> tfi_1\; \<local>\; t^k \; e^{*} : tfi_1$ because it is a premise of $S \vdash cl : tfi_1$.

        $S;C,\text{local } t_2^n\; t^k,\text{label }(ti_4^{m};l_4;g_4;\phi_4),\text{return }(ti_4^{m};l_4;g_4;\phi_4) \vdash e^{*}: tfi_2$ because it is a premise of the above derivation.

        $S;C,\text{local } t_2^n\; t^k,\text{return }(ti_4^{m};l_4;g_4;\phi_4) \vdash \<block> tfi_2\; e^{*} \<end> : tfi_2$ by $block$.

        There are now two cases, based on whether or not the called closure was in the current module being called:

        \begin{itemize}
            \item Case: $i=j$
                By $inversion$, $g_1=g_3$ and $g_2=g_4$, so we will use $g_1$ instead of $g_3$ and $g_2$ instead of $g_4$.

                $C \vdash_j v^n \; (t \<const> 0)^k : \epsilon;l_3;g_1;\phi_1 \rightarrow \ti{t_2}{a_2}^n\;\ti{t}{a}^k ;l_3;g_1;\phi_1,\ti{t_2}{a_2},(\<eq> a_2 \; \ti{t_2}{c})^n,\ti{t}{a},(\<eq> a \; \ti{t}{0})^k$ by $const$.

                $\phi_1,\ti{t_2}{a_2},(\<eq> a_2 \; \ti{t_2}{c})^n \implies \phi_3$, and therefore $\phi_1,\ti{t_2}{a_2},(\<eq> a_2 \; \ti{t_2}{c})^n,\ti{t}{a},(\<eq> a \; \ti{t}{0})^k \implies \phi_3,\ti{t}{a}^k,(\<eq> a \;\ti{t}{0})^k$.

                $S;C,\text{local } t_2^n\; t^k,\text{return }(ti_4^{m};l_4;g_2;\phi_4) \vdash \<block> tfi_2\; e^{*} \<end> :  ti_3^{n};\ti{t_2}{a_2}^{n}\; \ti{t}{a}^k;g_1;\phi_1,\ti{t_2}{a_2},(\<eq> a_2 \; \ti{t_2}{c})^n,\ti{t}{a},(\<eq> a \; \ti{t}{0})^k \rightarrow ti_4^{m};l_4;g_2;\phi_4$ by $sub-typing$.

                $S;(ti_4^{m};l_4;g_2;\phi_4) \vdash_j v^n \; (t \<const> 0)^k;\<block> tfi_2\; e^{*} \<end> : \epsilon;l_3;g_1;\phi_1 \rightarrow ti_4^{m};l_4;g_2;\phi_4$ by $with-return$.

                $S;C \vdash_i \<local>_m\{j;v^n \; (t.\<const> 0)^k\} \; \<block> tfi_2\; e^{*} \<end> \<end> : \epsilon;l_1;g_1;\phi_1 \rightarrow \epsilon\;ti_4^m;l_1;g_2;\phi_4$ by $local-same-inst$.

                $S;C \vdash_i \<local>_m\{j;v^n \; (t.\<const> 0)^k\} \; \<block> tfi_2\; e^{*} \<end> \<end> : tfi_0$ by $stack-poly$ and $sub-typing$.

            \item Case: $i \neq j$
                By $inversion$, $g_2=\ti{t_g}{a_3}^{*}$ where $C_\text{global}=(mut?\; t_g)^{*}$ and $a_3^{*}$ are fresh.

                $C \vdash_j v^n \; (t \<const> 0)^k : \epsilon;l_3;g_3;\phi_1 \rightarrow \ti{t_2}{a_2}^n\;\ti{t}{a}^k ;l_3;g_3;\phi_1,\ti{t_2}{a_2},(\<eq> a_2 \; \ti{t_2}{c})^n,\ti{t}{a},(\<eq> a \; \ti{t}{0})^k$ by $const$

                $\phi_1,\ti{t_2}{a_2},(\<eq> a_2 \; \ti{t_2}{c})^n \implies \phi_3$, and therefore $\phi_1,\ti{t_2}{a_2},(\<eq> a_2 \; \ti{t_2}{c})^n,\ti{t}{a},(\<eq> a \; \ti{t}{0})^k \implies \phi_3,\ti{t}{a}^k,(\<eq> a \;\ti{t}{0})^k$.

                $S;C,\text{local } t_2^n\; t^k,\text{return }(ti_4^{m};l_4;g_4;\phi_4) \vdash \<block> tfi_2\; e^{*} \<end> :  ti_3^{n};\ti{t_2}{a_2}^{n}\; \ti{t}{a}^k;g_3;\phi_1,\ti{t_2}{a_2},(\<eq> a_2 \; \ti{t_2}{c})^n,\ti{t}{a},(\<eq> a \; \ti{t}{0})^k \rightarrow ti_4^{m};l_4;g_4;\phi_4$ by $sub-typing$.

                $S;(ti_4^{m};l_4;g_4;\phi_4) \vdash_j v^n \; (t \<const> 0)^k;\<block> tfi_2\; e^{*} \<end> : \epsilon;l_3;g_3;\phi_1 \rightarrow ti_4^{m};l_4;g_4;\phi_4$ by $with-return$.

                $S;C \vdash_i \<local>_m\{j;v^n \; (t.\<const> 0)^k\} \; \<block> tfi_2\; e^{*} \<end> \<end> : \epsilon;l_1;g_1;\phi_1 \rightarrow \epsilon\;ti_4^m;l_1;\ti{t_g}{a_3}^{*};\phi_4$ by $local-diff-inst$.

                $S;C \vdash_i \<local>_m\{j;v^n \; (t.\<const> 0)^k\} \; \<block> tfi_2\; e^{*} \<end> \<end> : tfi_0$ by $stack-poly$ and $sub-typing$.
        \end{itemize}

    \item Case: $S;C \vdash \<local>_n \{ i;v_l^{*} \} \; v^n \<end> : ti_1^{*};l_1;\phi_1 \rightarrow ti_2^{*};l_2;\phi_2$
    \\ $\land$ $\<local>_n \{ i;v^{*}_l \} \; v^n \<end> \hookrightarrow_j \; v^n$

        By \reflemma{Inversion} on \refrule{Local}, $ti_2^{*} = ti_2^{*} \; ti^n$, $l_1 = l_2$,
        $S;(ti^n;l_3;\phi_3) \vdash_i v_l^{*};v^n : ti^n;l_3;\phi_3$,
        and $\phi_1,\phi_3 \implies \phi_2$.

        $(\vdash v_l : ti_l;\phi_l)^{*}$ and $S;C_l \vdash v^n : \epsilon:ti_l^{*};\phi_l^{*} \rightarrow ti^n;l_3;\phi_3$
        because they are premises of \refrule{Code} which we have assumed to hold.

        $\phi_l^{*} = \circ,\ti{t}{a}^{*},(= a\;\ti{t}{c})^{*}$ because it is a premise of \refrule{Admin-Const} which we have assumed to hold.

        By \reflemma{Inversion} on \refrule{Const}, $\phi_l^{*},\phi_v^n \implies \phi_3$.

        Since $a^{*}$ are fresh, $\phi_v^n \implies \phi_3$.

        \thought{Is this enough justification?}

        $S;C \vdash v^n : \epsilon;l_1;\phi_1 \rightarrow ti^n;l_2;\phi_1,\phi_v^n$ by \refrule{Const}.

        $S;C \vdash v^n : \epsilon;l_1;\phi_1 \rightarrow ti^n;l_2;\phi_1,\phi_3$ by \refrule{Implies}.

        $S;C \vdash v^n : \epsilon;l_1;\phi_1 \rightarrow ti^n;l_2;\phi_2$ by \refrule{Implies}.

        Therefore $S;C \vdash v^n : ti_1^{*};l_1;\phi_1 \rightarrow ti_2^{*};l_2;\phi_2$ by \refrule{Stack-Poly}.

    \item Case: $S;C \vdash \<local>_n \{ i;v_l^{*} \} \; \<trap> \<end> : ti_1^{*};l_1;\phi_1 \rightarrow ti_2^{*};l_2;\phi_2$
    \\ $\land$ $\<local>_n \{ i;v_l^{*} \} \; \<trap> \<end> \hookrightarrow \; \<trap>$

        Trivially, $S;C \vdash \<trap> : ti_1^{*};l_1;\phi_1 \rightarrow ti_2^{*};l_2;\phi_2$ by \refrule{Trap}.

    \item Case: $S;C \vdash \<local>_n \{ i;v_l^{*} \} \; L^k[v^n \; \<return>] \<end> : ti_1^{*};l_1;\phi_1 \rightarrow ti_2^{*};l_2;\phi_2$
    \\ $\land$ $\<local>_n \{ i;v_l^{*} \} \; L^k[v^n \; \<return>] \<end> \hookrightarrow_j \; v^n$

        By \reflemma{Inversion} on \refrule{Local}, $ti_2^{*} = ti_1^{*} \; ti^n$, $l_1 = l_2$,
        $S;(ti^n;l_3;\phi_3) \vdash_i v_l^{*};L^k[v^n \; \<return>] : ti^n;l_3;\phi_3$,
        and $\phi_1,\phi_3 \implies \phi_2$.

        $(\vdash v_l : ti_l;\phi_l)^{*}$ and $S;C_l \vdash L^k[v^n \; \<return>] : \epsilon;ti_l^{*};\phi_l^{*} \rightarrow ti^n;l_3;\phi_3$,
        where $C_l = S_\text{inst}(i),\text{local} \; t^{*}, \text{return} \; (ti^n;l_3;\phi_3)$,
        because they are premises of \refrule{Code} that we have assumed to hold.

        $ti_l^{*} = \ti{t_l}{a_l}^{*}$ because it is a premise of \refrule{Admin-Const} which we have assumed to hold.

        By \reflemma{Inversion} on \refrule{Composition},
        $C_l \vdash v^n : ti_4^{*};l_4;\phi_4 \rightarrow ti_5^{*};l_5;\phi_5$,
        and $C_l \vdash \<return> : ti_5^{*};l_5;\phi_5 \rightarrow ti_6^{*};l_6;\phi_6$.

        By \reflemma{Inversion} on \refrule{Return},
        $ti_5^{*} = ti_7^{*}\;ti^n$, $l_5 = l_3$, and $\phi_5 \implies \phi_3$.

        By \reflemma{Inversion} on \refrule{Const},
        $ti_5^{*} = ti_4^{*}\;ti^n$, $l_4 = l_5$,
        and $\phi_4,\phi_v^n \implies \phi_5$.

        $C_l \vdash v^n : \epsilon;l_3;\phi_4 \rightarrow ti^n;l_3;\phi_4,\phi_v^n$ by \refrule{Const}.

        $C_l \vdash v^n : \epsilon;ti_l^{*};\phi_l^{*} \rightarrow ti^n;l_3;\phi_4,\phi_v^n$ by \reflemma{Lift-Consts}.

        By \reflemma{Inversion} on \refrule{Const}, $\phi_l^{*} \implies \phi_4$.

        \thought{This is kinda non-obvious}

        Since $a_l^{*}$ are fresh, $\circ \implies \phi_4$.

        $C_l \vdash v^n : \epsilon;l_1;\phi_1 \rightarrow ti^n;l_2;\phi_1,\phi_v^n$ by \refrule{Const}.

        $C_l \vdash v^n : \epsilon;l_1;\phi_1 \rightarrow ti^n;l_2;\phi_1,\phi_3$ by \refrule{Implies}.

        \thought{This is using like 5 different implication arrows.}

        $C_l \vdash v^n : \epsilon;l_1;\phi_1 \rightarrow ti^n;l_2;\phi_2$ by \refrule{Implies}.

        Therefore, $C_l \vdash v^n : ti_1^{*};l_1;\phi_l^{*} \rightarrow ti_2^{*};l_2;\phi_2$ by \refrule{Stack-Poly}.

        \thought{There has to be a better way to do this proof...}

    \item Case: $S;\epsilon \vdash_i v_1^j\;v\;v_2^k;\<getlocal> j : ti^{*};l;\phi$
    \\ $\land$ $v_1^j\;v\;v_2^k;\<getlocal> j \hookrightarrow v$

        $\vdash v : \ti{t}{a};\phi_v$ and $S;C \vdash \<getlocal> j : \epsilon;l_1;\phi_1^j,\phi_v,\phi_2^k \rightarrow ti^{*};l;\phi$,
        because they are premises of \refrule{Code} that we have assumed to hold.

        $t.\<const> c = v$, and $\phi_v = \circ,\ti{t}{a},(= a\;\ti{t}{c})$, because it is a premise of \refrule{Admin-Const} that we have assumed to hold.

        By \reflemma{Inversion} on \refrule{Get-Local},
        $ti^{*} = \ti{t}{a_2}$, $l_1 = l$, and $\phi_1^j,\phi_v,\phi_2^k,\ti{t}{a_2},(= a_2\;a) \implies \phi$.

        $C \vdash v : \epsilon;l;\phi_1^j,\phi_v,\phi_2^k \rightarrow \ti{t}{a_2};l;\phi_1^j,\phi_v,\phi_2^k,\ti{t}{a_2},(= a_2\;\ti{t}{c})$ by \refrule{Const}.

        $\phi_v,\ti{t}{a_2},(= a_2\;\ti{t}{c}) \iff \phi_v,\ti{t}{a_2},(= a_2\;a)$ trivially.

        $C \vdash v : \epsilon;l;\phi_1^j,\phi_v,\phi_2^k \rightarrow \ti{t}{a_2};l;\phi$ by \refrule{Implies}.

        Therefore, $S;\epsilon \vdash_i v_1^j\;v\;v_2^k;v : ti^{*};l;\phi$ by \refrule{Code}.

    \item Case: $S;\epsilon \vdash_i v_1^j \; v \; v_2^k; v' \; (\<setlocal> j) : ti^{*};l;\phi$
    \\ $\land$ $v_1^j \; v \; v_2^k;v' \; \<setlocal> j \hookrightarrow v_1^j \; v' \; v_2^k;\epsilon$

        $\vdash v : \ti{t}{a};\phi_v$,
        $S;C \vdash v' \; (\<setlocal> j) : \epsilon:l_1;\phi_1^j,\phi_v,\phi_2^k \rightarrow ti^{*};l;\phi$,
        $l_1(j) = \ti{t}{a}$, and $C_\text{local}(j) = t$ because they are premises of \refrule{Code} that we have assumed to hold.

        $t.\<const> c = v$ and $\phi_v = \circ,\ti{t}{a},(= a\;\ti{t}{c})$ because they are premises of \refrule{Admin-Const} that we have assumed to hold.

        By \reflemma{Inversion} on \refrule{Composition},
        $C \vdash v' : \epsilon;l_1;\phi_1^j,\phi_v,\phi_2^k \rightarrow ti_3^{*};l_3;\phi_3$,
        $C \vdash \<setlocal> j : ti_3^{*};l_3;\phi_3 \rightarrow ti^{*};l;\phi$.

        Recalling that $t = C_\text{local}(j)$;
        by \reflemma{Inversion} on \refrule{Set-Local},
        $ti_3^{*} = ti^{*} \; \ti{t}{a'}$,
        $l = l_3[j := \ti{t}{a'}]$,
        and $\phi_3 \implies \phi$.

        By \reflemma{Inversion} on \refrule{Const},
        $t.\<const> c' = v'$, $ti^{*} = \epsilon$, $l_1 = l_3$, and\\
        $\phi_1^j,\phi_v,\phi_2^k,\ti{t}{a'},(= a'\;\ti{t}{c'}) \implies \phi_3$.

        $C \vdash \epsilon : \epsilon;l;\phi \rightarrow \epsilon;l;\phi$ by \refrule{Empty}.

        $C \vdash \epsilon : \epsilon;l;\phi_1^j,\phi_v,\phi_2^k,\ti{t}{a'},(= a'\;\ti{t}{c'}) \rightarrow \epsilon;l;\phi$ by \refrule{Implies}.

        % Since $a$ is fresh in the typing derivation, $C \vdash \epsilon : \epsilon;l;\phi_1^j,\phi_2^k,\ti{t}{a'},(= a'\;\ti{t}{c'}) \rightarrow \epsilon;l;\phi$.

        Since $a$ is fresh, $\phi_1^j,\phi_2^k,\ti{t}{a'},(= a'\;\ti{t}{c'}) \implies \phi_1^j,\phi_v,\phi_2^k,\ti{t}{a'},(= a'\;\ti{t}{c'})$.

        $C \vdash \epsilon : \epsilon;l;\phi_1^j,\phi_2^k,\ti{t}{a'},(= a'\;\ti{t}{c'}) \rightarrow \epsilon;l;\phi$ by \refrule{Implies}.

        $\vdash v' : \ti{t}{a'};\circ,\ti{t}{a'},(= a'\;\ti{t}{c'})$ by \refrule{Admin-Const}.

        Therefore, $S;\epsilon \vdash_i v_1^j\;v'\;v_2^k;\epsilon : ti^n;l;\phi$ by \refrule{Code}.

        \thought{I set out to write a very verbose proof case, but I didn't expect it to be this verbose.}

    \item Case: $C \vdash v \; (\<teelocal> j) : ti_1^{*};l_1;\phi_1 \rightarrow ti_2^{*};l_2;\phi_2$
    \\ $\land$ $v \; (\<teelocal> j) \hookrightarrow v\;v\;(\<setlocal> j)$

        By \reflemma{Inversion} on \refrule{Composition},
        $C \vdash v : ti_1^{*};l_1;\phi_1 \rightarrow ti_3^{*};l_3;\phi_3$,
        and $C \vdash \<teelocal> j : ti_3^{*};l_3;\phi_3 \rightarrow ti_2^{*};l_2;\phi_2$.

        By \reflemma{Inversion} on \refrule{Tee-Local},
        $ti_3^{*} = ti^{*} \; \ti{t}{a}$, $ti_2^{*} = ti^{*} \; \ti{t}{a_2}$, $l_2 = l_3[j := \ti{t}{a}]$,
        and $\phi_3,\ti{t}{a_2},(= a_2\;a) \implies \phi_2$.

        By \reflemma{Inversion} on \refrule{Const},
        $t.\<const> c = v$, $ti_1^{*} = ti^{*}$, $l_3 = l_1$,
        and $\phi_1,\ti{t}{a},(= a\;\ti{t}{c}) \implies \phi_3$.

        $C \vdash v\;v : \epsilon;l_1;\phi_1 \rightarrow \ti{t}{a_2}\;\ti{t}{a};l_1;\phi_1,\ti{t}{a_2},(= a_2\;\ti{t}{c}),\ti{t}{a},(= a\;\ti{t}{c})$ by \refrule{Const}.

        $\ti{t}{a_2},(= a_2\;\ti{t}{c}),\ti{t}{a},(= a\;\ti{t}{c}) \iff \ti{t}{a_2},(= a_2\;a),\ti{t}{a},(= a\;\ti{t}{c})$ trivially.

        $C \vdash v\;v : \epsilon;l_1;\phi_1 \rightarrow \ti{t}{a_2}\;\ti{t}{a};l_1;\phi_2$ by \refrule{Implies}.

        $C \vdash \<setlocal> j : \ti{t}{a};l_1;\phi_2 \rightarrow \epsilon;l_1[j := \ti{t}{a}];\phi_2$ by \refrule{Set-Local}.

        Therefore, $C \vdash v\;v\;(\<setlocal> j) : ti_1^{*};l_1;\phi_1 \rightarrow ti_2^{*};l_2;\phi_2$ by \refrule{Composition} and \refrule{Stack-Poly}.

    \item Case: $C \vdash \<getglobal> j : ti_1^{*};l_1;\phi_1 \rightarrow ti_2^{*};l_2;\phi_2$
    \\ $\land$ $s;\<getglobal> j \hookrightarrow_i s_\text{glob}(i,j)$

        $\vdash s : S$ and $S;\epsilon \vdash_i v^{*};\<getglobal> j : ti^{*};l;\phi$ because they are premises of \refrule{Program} that we have assumed to hold.

        $S;C \vdash \<getglobal> j : \epsilon;l_1;\phi_v^{*} \rightarrow ti^{*};l;\phi$ because it is a premise of \refrule{Code} that we have assumed to hold.

        By \reflemma{Inversion} on \refrule{Get-Global}, $ti^{*} = \ti{t}{a}$, $l = l_1$, $C_\text{global}(j) = \text{mut}^{?} t$,
        and $\phi_v^{*},\ti{t}{a} \implies \phi$.

        $S \vdash s_\text{inst}(i) : C$ because it is a premise of \refrule{Store} that we have assumed to hold.

        Recalling that $C_\text{global}(j) = \text{mut}^{?} t$;
        $\vdash s_\text{glob}(i,j) : \ti{t}{a_1};\phi_1$ because it is a premise of \refrule{Instance} that we have assumed to hold.

        $S;C \vdash t.\<const> c : \epsilon;l;\phi_v^{*} \rightarrow \ti{t}{a};l;\phi_v^{*},\ti{t}{a},(= a \; \ti{t}{c})$ by \refrule{Const},
        where $t.\<const> c = s_\text{glob}(i,j)$.

        $\ti{t}{a},(= a\;\ti{t}{c}) \implies \ti{t}{a}$ trivially.

        $S;C \vdash s_\text{glob}(i,j) : \epsilon;l;\phi_v^{*} \rightarrow \ti{t}{a};l;\phi$ by \refrule{Implies}.

        $S;\epsilon \vdash_i v^{*};s_\text{glob}(i,j) : \ti{t}{a};l;\phi$ by \refrule{Code}, having assumed that the other premises hold.

        \todo{Phrase this better.}

        Therefore, $\vdash_i s;v^{*};s_\text{glob}(i,j) : \ti{t}{a};l;\phi$ by \refrule{Program}.

    \item Case: $\vdash_i s;v_l^{*};v \; (\<setglobal> j) : ti^{*};l;\phi$
    \\ $\land$ $s;v \; (\<setglobal> j) \hookrightarrow_i s';\epsilon$, where $s' = s$ with $\text{glob}(i,j) = v$

        $\vdash s : S$ and $S;\epsilon \vdash_i v_l^{*};v \; (\<setglobal> j) : ti^{*};l;\phi$ because they are premises of \refrule{Program} that we have assumed to hold.

        $S;C \vdash v \; (\<setglobal> j) : \epsilon;l_1;\phi_1 \rightarrow ti^{*};l;\phi$ because it is a premise of \refrule{Code} that we have assumed to hold.

        By \reflemma{Inversion} on \refrule{Composition}, \refrule{Set-Global}, and \refrule{Const},
        $t.\<const> c = v$, $ti^{*} = \epsilon$, $l_1 = l$, $C_\text{global}(j) = \text{mut}\;t$,
        and $\phi_1,\ti{t}{a},(= a\;\ti{t}{c}) \implies \phi$.

        % By \reflemma{Inversion} on \refrule{Composition},
        % $C \vdash v : \epsilon;l_1;\phi_1 \rightarrow ti_2^{*};l_2;\phi_2$,
        % and $C \vdash \<setglobal> j : ti_2^{*};l_2;\phi_2 \rightarrow ti^{*};l;\phi$.

        % By \reflemma{Inversion} on \refrule{Set-Global},
        % $ti_2^{*} = ti^{*} \; \ti{t}{a}$, $l_2 = l$, $C_\text{global}(j) = \text{mut}\;t$,
        % and $\phi_2, \implies \phi$.

        % By \reflemma{Inversion} on \refrule{Const},
        % $t.\<const> c = v$, $ti_2^{*} = \ti{t}{a}$, $l_1 = l_2$,
        % and $\phi_1,\ti{t}{a},(= a\;\ti{t}{c}) \implies \phi_2$.

        $S;C \vdash \epsilon : \epsilon;l;\phi \rightarrow \epsilon;l;\phi$ by \refrule{Empty}.

        Since $a$ is fresh, $\phi_1 \implies \phi_1,\ti{t}{a},(= a\;\ti{t}{c})$.

        $S;C \vdash \epsilon : \epsilon;l;\phi_1 \rightarrow \epsilon;l;\phi$ by \refrule{Implies}.

        $S;\epsilon \vdash_i v_l^{*};\epsilon : ti^{*};l;\phi$ by \refrule{Code}.

        $S \vdash s_\text{inst}(i) : C$ because it is a premise of \refrule{Store} that we have assumed to hold.

        $\vdash s_\text{glob}(i,j) : \ti{t}{a_g};\phi_g$ because it is a premise of \refrule{Instance} that we have assumed to hold.

        $s' : S$ by \refrule{Instance} and \refrule{Store}.

        \thought{This might be skipping too much.}

        Therefore, $\vdash s';\epsilon : ti^{*};l;\phi$ by \refrule{Program}.

    \item Case: $\vdash_i s;v^{*};(\<ithreetwo>.\<const> k)\;(t.\<load> align\;o) : ti^{*};l;\phi$
    \\ $\land$ $s;(\<ithreetwo>.\<const> k)\;(t.\<load> align\;o) \hookrightarrow_i s;t.\<const> \text{const}_t(b^{*})$, where $s_\text{mem}(i,k+o,|t|) = b^{*}$

        $S;\epsilon \vdash_i v^{*};(\<ithreetwo>.\<const> k)\;(t.\<load> align\;o) : ti^{*};l;\phi$ and $\vdash s : S$ because they are premises of \refrule{Program} which we have assumed to hold.

        $S;C \vdash (\<ithreetwo>.\<const> k)\;(t.\<load> align\;o) : \epsilon;l_1;\phi_1 \rightarrow ti^{*};l;\phi$ because it is a premise of \refrule{Code} which we have assumed to hold.

        By \reflemma{Inversion} on \refrule{Composition}, \refrule{Const}, \refrule{Mem-Load},
        $ti^{*} = \ti{t}{a}$, $l_1 = l$, and $\phi_1,\ti{t}{a} \implies \phi$.

        $C \vdash t.\<const> \text{const}_t(b^{*}) : \epsilon;l;\phi_1 \rightarrow \ti{t}{a};l;\phi_1,\ti{t}{a},(= a\;\ti{t}{c})$ by \refrule{Const}.

        $C \vdash t.\<const> \text{const}_t(b^{*}) : \epsilon;l;\phi_1 \rightarrow \ti{t}{a};l;\phi$ by \refrule{Implies}.

        $S;\epsilon \vdash_i v^{*};t.\<const> \text{const}_t(b^{*}) : ti^{*};l;\phi$ by \refrule{Code}.

        Therefore, $s;t.\<const> \text{const}_t(b^{*}) : ti^{*};l;\phi$ by \refrule{Program}.

    \item Case: $\vdash_i s;v^{*};(\<ithreetwo>.\<const> k)\;(t.\<load> tp_sx\;align\;o) : ti^{*};l;\phi$
    \\ $\land$ $s;(\<ithreetwo>.\<const> k)\;(t.\<load> tp_sx\;align\;o) \hookrightarrow_i s;t.\<const> \text{const}_t^{sx}(b^{*})$, where $s_\text{mem}(i,k+o,|tp|) = b^{*}$

        Similar to \refrule{Mem-Load} non-packed.

    \item Case: $C \vdash (\<ithreetwo>.\<const> k)\;(t.\<load> tp\_sx^{?}\;align\;o) : ti_1^{*};l_1;\phi_1 \rightarrow ti_2^{*};l_2;\phi_2$
    \\ $\land$ $s;(\<ithreetwo>.\<const> k)\;(t.\<load> tp\_sx^{?}\;align\;o) \hookrightarrow_i \<trap>$

        Trivially, $C \vdash \<trap> : ti_1^{*};l_1;\phi_1 \rightarrow ti_2^{*};l_2;\phi_2$ by \refrule{Trap}.

    \item Case: $\vdash_i s;v^{*};(\<ithreetwo>.\<const> k)\;(t.\<const> c)\;(t.\<store> align\;o) : ti^{*};l;\phi$
    \\ $\land$ $s;(\<ithreetwo>.\<const> k)\;(t.\<const> c)\;(t.\<store> align\;o) \hookrightarrow_i s';\epsilon$, where $s' = s \text{ with } \text{mem}(i,k+o,|t|) = \text{bits}_t^{|t|}(c)$

        $S;\epsilon \vdash_i v^{*};(\<ithreetwo>.\<const> k)\;(t.\<const> c)\;(t.\<store> align\;o) : ti^{*};l;\phi$ and $\vdash s : S$ because they are premises of \refrule{Program} which we have assumed to hold.

        $S;C \vdash (\<ithreetwo>.\<const> k)\;(t.\<const> c)\;(t.\<store> align\;o) : \epsilon;l_1;\phi_1 \rightarrow ti^{*};l;\phi$ because it is a premise of \refrule{Code} which we have assumed to hold.

        By \reflemma{Inversion} on \refrule{Composition}, \refrule{Const}, and \refrule{Mem-Store},
        $ti^{*} = \epsilon$, $l_1 = l$, and $\phi_1,\ti{\<ithreetwo>}{a_1},(= a_1\;\ti{\<ithreetwo>}{k}),\ti{t}{a_2},(= a_2\;\ti{t}{c}) \implies \phi$.

        Since $a_1$ and $a_2$ are fresh, $\phi_1 \implies \phi$.

        $C \vdash \epsilon : \epsilon;l;\phi_1 \rightarrow \epsilon;l;\phi_1$ by \refrule{Empty}.

        $C \vdash \epsilon : \epsilon;l;\phi_1 \rightarrow \epsilon;l;\phi$ by \refrule{Implies}.

        $s' : S$ trivially.

        \thought{Maybe justify more? Intuitively the contents of the mem function doesn't affect the store typing.}

        $S;\epsilon \vdash_i v^{*};\epsilon : ti^{*};l;\phi$ by \refrule{Code}.

        Therefore, $\vdash_i s';\epsilon : ti^{*};l;\phi$ by \refrule{Program}.

    \item Case: $C \vdash (\<ithreetwo>.\<const> k)\;(t.\<const> c)\;(t.\<store> tp\;align\;o) : ti_1^{*};l_1;\phi_1 \rightarrow ti_2^{*};l_2;\phi_2$
    $\land$ $\vdash s : S$
    \\ $\land$ $s;(\<ithreetwo>.\<const> k)\;(t.\<const> c)\;(t.\<store> tp\;align\;o) \hookrightarrow_i s';\epsilon$, where $s' = s \text{ with } \text{mem}(i,k+o,|tp|)=\text{bits}_t^{|tp|}(c)$

        Similar to \refrule{Mem-Store} non-packed.

    \item Case: $C \vdash (\<ithreetwo>.\<const> k)\;(t.\<const> c)\;(t.\<store> tp^{?}\;align\;o) : ti_1^{*};l_1;\phi_1 \rightarrow ti_2^{*};l_2;\phi_2$
    \\ $\land$ $s;(\<ithreetwo>.\<const> k)\;(t.\<const> c)\;(t.\<store> tp^{?}\;align\;o) \hookrightarrow_i \<trap>$

        Trivially, $C \vdash \<trap> : ti_1^{*};l_1;\phi_1 \rightarrow ti_2^{*};l_2;\phi_2$ by \refrule{Trap}.

    \item Case: $\vdash_i s;v^{*};\<currentmemory> : ti^{*};l;\phi$
    \\ $\land$ $s;\<currentmemory> \hookrightarrow_i \<ithreetwo>.\<const> |s_\text{mem}(i,*)|/64\text{Ki}$

        $S;\epsilon \vdash_i v^{*};\<currentmemory> : ti^{*};l;\phi$, and $\vdash s : S$ because they are premises of \refrule{Program} which we have assumed to hold.

        $S;C \vdash \<currentmemory> : \epsilon;l_1;\phi_1 \rightarrow ti^{*};l;\phi$ because it is a premise of \refrule{Code} which we have assumed to hold.

        By \reflemma{Inversion} on \refrule{Current-Memory}, $ti^{*} = \ti{\<ithreetwo>}{a}$, $l_1 = l$, and $\phi_1,\ti{\<ithreetwo>}{a} \implies \phi$.

        Let $c = |s_\text{mem}(i,*)|/64\text{Ki}$.

        $S;C \vdash \<ithreetwo>.\<const> c : \epsilon;l;\phi_1 \rightarrow \ti{\<ithreetwo>}{a};l;\phi_1,\ti{\<ithreetwo>}{a},(= a\;\ti{\<ithreetwo>}{c})$ by \refrule{Const}.

        $S;C \vdash \<ithreetwo>.\<const> c : \epsilon;l;\phi_1 \rightarrow \ti{\<ithreetwo>}{a};l;\phi$ by \refrule{Implies}.

        $S;\epsilon \vdash_i v^{*};\<ithreetwo>.\<const> c : ti^{*};l;\phi$ by \refrule{Code}.

        Therefore, $\vdash_i s;\<ithreetwo>.\<const> |s_\text{mem}(i,*)|/64\text{Ki} : ti^{*};l;\phi$ by \refrule{Program}.

    \item Case: $\vdash_i s;v^{*};(\<ithreetwo>.\<const> k) \; \<growmemory> : ti^{*};l;\phi$
    \\ $\land$ $s;(\<ithreetwo>.\<const> k) \; \<growmemory> \hookrightarrow_i s';\<ithreetwo>.\<const> |s_\text{mem}(i,*)|/64\text{Ki}$, where $s' = s \text{ with } \text{mem}(i,*) = s_\text{mem}(i,*)(0)^{k \cdot 64\text{Ki}}$

        $S;\epsilon \vdash_i v^{*};(\<ithreetwo>.\<const> k) \; \<growmemory> : ti^{*};l;\phi$, and $\vdash s : S$ because they are premises of \refrule{Program} which we have assumed to hold.

        $S;C \vdash (\<ithreetwo>.\<const> k) \; \<growmemory> : \epsilon;l_1;\phi_1 \rightarrow ti^{*};l;\phi$ because it is a premise of \refrule{Code} which we have assumed to hold.

        By \reflemma{Inversion} on \refrule{Composition}, \refrule{Const}, and \refrule{Grow-Memory},
        $ti^{*} = \ti{\<ithreetwo>}{a_1}$, $l_1 = l$, and $\phi_1,\ti{\<ithreetwo>}{a_2},(= a_2\;\ti{\<ithreetwo>}{k}),\ti{\<ithreetwo>}{a_1} \implies \phi$.

        Since $a_2$ is fresh, $\phi_1,\ti{\<ithreetwo>}{a_1} \implies \phi$.

        $S_\text{mem}(i) \leq |s_\text{mem}(i,*)|$ because it is a premise of \refrule{Store} on $\vdash s : S$ which we have assumed to hold.

        $s' : S$ by \refrule{Store}, using $S_\text{mem}(i) \leq |s_\text{mem}(i,*)(0)^{k \cdot 64\text{Ki}}|$.

        \thought{Maybe explicitly lay out the $\leq$ relationship we're using?}

        Let $c = \<ithreetwo>.\<const> |s_\text{mem}(i,*)|/64\text{Ki}$.

        $C \vdash \<ithreetwo>.\<const> c : \epsilon;l;\phi_1 \rightarrow \ti{\<ithreetwo>}{a_1};l;\phi_1,\ti{\<ithreetwo>}{a_1},(= a_1\;\ti{\<ithreetwo>}{c})$ by \refrule{Const}.

        $C \vdash \<ithreetwo>.\<const> c : \epsilon;l;\phi_1 \rightarrow \ti{\<ithreetwo>}{a_1};l;\phi$ by \refrule{Implies}.

        $S;\epsilon \vdash_i \<ithreetwo>.\<const> c : ti^{*};l;\phi$ by \refrule{Code}.

        Therefore, $\vdash_i s';\<ithreetwo>.\<const> |s_\text{mem}(i,*)|/64\text{Ki} : ti^{*};l;\phi$ by \refrule{Program}.

    \item Case: $\vdash_i s;v^{*};(\<ithreetwo>.\<const> k) \; \<growmemory> : ti^{*};l;\phi$
    \\ $\land$ $s;(\<ithreetwo>.\<const> k) \; \<growmemory> \hookrightarrow_i \<ithreetwo>.\<const> (-1)$

        $S;\epsilon \vdash_i v^{*};(\<ithreetwo>.\<const> k) \; \<growmemory> : ti^{*};l;\phi$, and $\vdash s : S$ because they are premises of \refrule{Program} which we have assumed to hold.

        $S;C \vdash (\<ithreetwo>.\<const> k) \; \<growmemory> : \epsilon;l_1;\phi_1 \rightarrow ti^{*};l;\phi$ because it is a premise of \refrule{Code} which we have assumed to hold.

        By \reflemma{Inversion} on \refrule{Composition}, \refrule{Const}, \refrule{Grow-Memory},
        $ti^{*} = \ti{\<ithreetwo>}{a_1}$, $l_1 = l$, and $\phi_1,\ti{\<ithreetwo>}{a_2},(= a_2\;\ti{\<ithreetwo>}{k}),\ti{\<ithreetwo>}{a_1} \implies \phi$.

        Since $a_2$ is fresh, $\phi_1,\ti{\<ithreetwo>}{a_1} \implies \phi$.

        $C \vdash \<ithreetwo>.\<const> (-1) : \epsilon;l;\phi_1 \rightarrow \ti{\<ithreetwo>}{a_1};l;\phi_1,\ti{\<ithreetwo>}{a_1},(= a_1\;\ti{\<ithreetwo>}{(-1)})$ by \refrule{Const}.

        $C \vdash \<ithreetwo>.\<const> (-1) : \epsilon;l;\phi_1 \rightarrow \ti{\<ithreetwo>}{a_1};l;\phi$ by \refrule{Implies}.

        $S;\epsilon \vdash_i \<ithreetwo>.\<const> (-1) : ti^{*};l;\phi$ by \refrule{Code}.

        Therefore, $\vdash_i s;\<ithreetwo>.\<const> (-1) : ti^{*};l;\phi$ by \refrule{Program}.

\end{itemize}
\end{proof}
